Basic support for n-ary tuples (#1)

Examples/tuples.ml
@@ -1,0 +1,12 @@
+(* Functions that use tuples as arguments or return values. *)
+
+(* 1. Swap a pair: returns (b, a) given (a, b) as ints *)
+let swap_pair (p: int * int) : int * int =
+  let a = p.0  in
+  let b = p.1 in
+  (b, a)
+[@@spec fun p ->
+  ret (fun v ->
+    assert (p.0 = v.1);
+    assert (p.1 = v.0);
+    ret ())];;
